theories/CodegenWasm/LambdaANF_to_Wasm_primitives.v
@@ -1,23 +1,58 @@
-From Wasm Require Import datatypes operations.
-From CertiCoq Require Import LambdaANF.toplevel LambdaANF.cps_util.
+From Coq Require Import POrderedType ZArith BinNat List Lia Uint63.
+From Wasm Require Import datatypes operations numerics.
+Import Wasm_int.
 
-From CertiCoq Require Import Common.Common Common.compM Common.Pipeline_utils.
+Require Import compcert.lib.Coqlib.
+
+From CertiCoq Require Import
+  LambdaANF.toplevel LambdaANF.cps_util LambdaANF.cps LambdaANF.cps_show
+  Common.Common Common.compM Common.Pipeline_utils.
+
 Require Import ExtLib.Structures.Monad.
-From MetaCoq.Utils Require Import bytestring MCString.
-From Coq Require Import ZArith BinNat List Lia.
+From MetaCoq Require Import Common.Kernames Utils.bytestring Utils.MCString.
 
-Require Import MSets.MSetAVL.
-From Coq Require Import FMapAVL.
-Require Import POrderedType.
+Import ssreflect MonadNotation SigTNotations.
 
-Require Import LambdaANF.cps LambdaANF.cps_show.
-Import MonadNotation.
+Notation "'primInt' x" := (AstCommon.primInt ; x) (at level 0).
 
-Definition nat_to_i32val n :=
-  VAL_int32 (Wasm_int.Int32.repr (BinInt.Z.of_nat n)).
+(* Define convenience wrappers as notations to allow easy unfolding during proofs *)
+Notation uint63 := Uint63.int.
+Notation Z_to_i64 z := (Int64.repr z).
+Notation Z_to_VAL_i64 z := (VAL_int64 (Int64.repr z)).
+Notation nat_to_VAL_i32 n := (VAL_int32 (Wasm_int.Int32.repr (BinInt.Z.of_nat n))).
+Notation N_to_VAL_i32 n := (VAL_int32 (Wasm_int.Int32.repr (BinInt.Z.of_N n))).
 
-Definition nat_to_i64val n :=
-  VAL_int64 (Wasm_int.Int64.repr (BinInt.Z.of_nat n)).
+Local Coercion Z_to_i64_co z := Z_to_i64 z.
+Local Coercion Z_to_i64val_co z := Z_to_VAL_i64 z.
+
+(* Avoid unfolding during proofs *)
+Opaque Uint63.to_Z.
+
+
+
+
+
+Section TRANSLATION.
+
+Variables global_mem_ptr glob_tmp1 glob_tmp2 glob_tmp3 glob_tmp4 : globalidx.
+
+Definition maxuint31 := 2147483647%Z.
+Definition maxuint63 := 9223372036854775807%Z.
+
+
+(* Ordinals of constructors *)
+Definition true_ord  := 0%N.
+Definition false_ord := 1%N.
+
+Definition Eq_ord    := 0%N.
+Definition Lt_ord    := 1%N.
+Definition Gt_ord    := 2%N.
+
+Definition C0_ord    := 0%N.
+Definition C1_ord    := 1%N.
+
+Definition pair_ord  := 0%N.
+
 
 (* **** TRANSLATE PRIMITIVE VALUES **** *)
 
@@ -26,516 +61,486 @@ Definition translate_primitive_value (p : AstCommon.primitive) : error Wasm_int.
   | AstCommon.primInt => fun i => Ret (Wasm_int.Int64.repr (Uint63.to_Z i))
   | AstCommon.primFloat => fun f => Err "Extraction of floats to Wasm not yet supported"
   end (projT2 p).
-  
+
 (* **** TRANSLATE PRIMITIVE OPERATIONS **** *)
 
-Section PrimitiveOperators.
-
-Variables global_mem_ptr glob_tmp1 glob_tmp2 glob_tmp3 glob_tmp4 : globalidx.
-
+(* Path of the PrimInt63 module in the kernel: Coq.Numbers.Cyclic.Int63.PrimInt63 *)
 Definition primInt63ModPath : Kernames.modpath :=
   Kernames.MPfile [ "PrimInt63"%bs ; "Int63"%bs ; "Cyclic"%bs ; "Numbers"%bs ; "Coq"%bs ].
 
-Definition primInt63Add        : Kernames.kername := (primInt63ModPath, "add"%bs).
-Definition primInt63Addc       : Kernames.kername := (primInt63ModPath, "addc"%bs).
-Definition primInt63Addcarryc  : Kernames.kername := (primInt63ModPath, "addcarryc"%bs).
-Definition primInt63Sub        : Kernames.kername := (primInt63ModPath, "sub"%bs).
-Definition primInt63Subc       : Kernames.kername := (primInt63ModPath, "subc"%bs).
-Definition primInt63Subcarryc  : Kernames.kername := (primInt63ModPath, "subcarryc"%bs).
-Definition primInt63Mul        : Kernames.kername := (primInt63ModPath, "mul"%bs).
-Definition primInt63Mulc       : Kernames.kername := (primInt63ModPath, "mulc"%bs).
-Definition primInt63Div        : Kernames.kername := (primInt63ModPath, "div"%bs).
-Definition primInt63Mod        : Kernames.kername := (primInt63ModPath, "mod"%bs).
-Definition primInt63Land       : Kernames.kername := (primInt63ModPath, "land"%bs).
-Definition primInt63Lor        : Kernames.kername := (primInt63ModPath, "lor"%bs).
-Definition primInt63Lxor       : Kernames.kername := (primInt63ModPath, "lxor"%bs).
-Definition primInt63Lsl        : Kernames.kername := (primInt63ModPath, "lsl"%bs).
-Definition primInt63Lsr        : Kernames.kername := (primInt63ModPath, "lsr"%bs).
-Definition primInt63Compare    : Kernames.kername := (primInt63ModPath, "compare"%bs).
-Definition primInt63Eqb        : Kernames.kername := (primInt63ModPath, "eqb"%bs).
-Definition primInt63Ltb        : Kernames.kername := (primInt63ModPath, "ltb"%bs).
-Definition primInt63Leb        : Kernames.kername := (primInt63ModPath, "leb"%bs).
-Definition primInt63Head0      : Kernames.kername := (primInt63ModPath, "head0"%bs).
-Definition primInt63Tail0      : Kernames.kername := (primInt63ModPath, "tail0"%bs).
-Definition primInt63Addmuldiv  : Kernames.kername := (primInt63ModPath, "addmuldiv"%bs).
-Definition primInt63Diveucl    : Kernames.kername := (primInt63ModPath, "diveucl"%bs).
-Definition primInt63Diveucl_21 : Kernames.kername := (primInt63ModPath, "diveucl_21"%bs).
+(* Supported operators defined as data type to avoid pattern matching on kernel name (bytestrings) *)
+Inductive primop :=
+| PrimInt63add
+| PrimInt63sub
+| PrimInt63mul
+| PrimInt63div
+| PrimInt63mod
+| PrimInt63lsl
+| PrimInt63lsr
+| PrimInt63land
+| PrimInt63lor
+| PrimInt63lxor
+| PrimInt63eqb
+| PrimInt63ltb
+| PrimInt63leb
+| PrimInt63compare
+| PrimInt63addc
+| PrimInt63addcarryc
+| PrimInt63subc
+| PrimInt63subcarryc
+| PrimInt63mulc
+| PrimInt63head0
+| PrimInt63tail0
+| PrimInt63diveucl
+| PrimInt63diveucl_21
+| PrimInt63addmuldiv.
 
-Definition maxuint31 := VAL_int64 (Wasm_int.Int64.repr 2147483647%Z).
-Definition maxuint63 := VAL_int64 (Wasm_int.Int64.repr 9223372036854775807%Z).
+Definition primop_map : KernameMap.t primop :=
+  KernameMap.add (primInt63ModPath, "add") PrimInt63add
+    (KernameMap.add (primInt63ModPath, "sub") PrimInt63sub
+    (KernameMap.add (primInt63ModPath, "mul") PrimInt63mul
+    (KernameMap.add (primInt63ModPath, "div") PrimInt63div
+    (KernameMap.add (primInt63ModPath, "mod") PrimInt63mod
+    (KernameMap.add (primInt63ModPath, "lsl") PrimInt63lsl
+    (KernameMap.add (primInt63ModPath, "lsr") PrimInt63lsr
+    (KernameMap.add (primInt63ModPath, "land") PrimInt63land
+    (KernameMap.add (primInt63ModPath, "lor") PrimInt63lor
+    (KernameMap.add (primInt63ModPath, "lxor") PrimInt63lxor
+    (KernameMap.add (primInt63ModPath, "eqb") PrimInt63eqb
+    (KernameMap.add (primInt63ModPath, "ltb") PrimInt63ltb
+    (KernameMap.add (primInt63ModPath, "leb") PrimInt63leb
+    (KernameMap.add (primInt63ModPath, "compare") PrimInt63compare
+    (KernameMap.add (primInt63ModPath, "addc") PrimInt63addc
+    (KernameMap.add (primInt63ModPath, "addcarryc") PrimInt63addcarryc
+    (KernameMap.add (primInt63ModPath, "subc") PrimInt63subc
+    (KernameMap.add (primInt63ModPath, "subcarryc") PrimInt63subcarryc
+    (KernameMap.add (primInt63ModPath, "mulc") PrimInt63mulc
+    (KernameMap.add (primInt63ModPath, "head0") PrimInt63head0
+    (KernameMap.add (primInt63ModPath, "tail0") PrimInt63tail0
+    (KernameMap.add (primInt63ModPath, "diveucl") PrimInt63diveucl
+    (KernameMap.add (primInt63ModPath, "diveucl_21") PrimInt63diveucl_21
+    (KernameMap.add (primInt63ModPath, "addmuldiv") PrimInt63addmuldiv
+    (KernameMap.empty primop)))))))))))))))))))))))).
 
 Definition load_local_i64 (i : localidx) : list basic_instruction :=
   [ BI_local_get i ; BI_load T_i64 None 2%N 0%N ].
 
 Definition increment_global_mem_ptr i :=
   [ BI_global_get global_mem_ptr
-  ; BI_const_num (nat_to_i32val i)
+  ; BI_const_num (nat_to_VAL_i32 i)
   ; BI_binop T_i32 (Binop_i BOI_add)
   ; BI_global_set global_mem_ptr
   ].
 
-Definition apply_binop_and_store_i64 (op : list basic_instruction) x y :=
-  BI_global_get global_mem_ptr :: (* Address to store the result of the operation *)
-  load_local_i64 x ++             (* Load the arguments onto the stack *)
+Definition bitmask_instrs := [ BI_const_num maxuint63 ; BI_binop T_i64 (Binop_i BOI_and) ].
+
+Definition apply_binop_and_store_i64 (op : binop_i) (x y : localidx) (apply_bitmask : bool) : list basic_instruction :=
+  BI_global_get global_mem_ptr ::                   (* Address to store the result of the operation *)
+  load_local_i64 x ++                               (* Load the arguments onto the stack *)
   load_local_i64 y ++
-  op ++
-  [ BI_store T_i64 None 2%N 0%N   (* Store the result *)
-  ; BI_global_get global_mem_ptr  (* Put the address where the result was stored on the stack *)
+  [ BI_binop T_i64 (Binop_i op) ] ++
+  (if apply_bitmask then bitmask_instrs else []) ++ (* apply bitmask to zero MSB if necessary *)
+  [ BI_store T_i64 None 2%N 0%N                     (* Store the result *)
+  ; BI_global_get global_mem_ptr                    (* Put the result address on the stack *)
   ] ++
   increment_global_mem_ptr 8.
 
-Definition make_carry (ord : nat) (gidx : globalidx) : list basic_instruction:=
+(* Assume argument is stored in global gidx *)
+Definition make_carry (ord : N) (gidx : globalidx) : list basic_instruction:=
   [ BI_global_get global_mem_ptr
   ; BI_global_get gidx
   ; BI_store T_i64 None 2%N 0%N
   ; BI_global_get global_mem_ptr
-  (* ; BI_const_num (nat_to_i32val 8) *)
-  (* ; BI_binop T_i32 (Binop_i BOI_add) *)
-  (* ; BI_global_set constr_alloc_ptr *)
-  (* ; BI_global_get constr_alloc_ptr *)
-  ; BI_const_num (nat_to_i32val ord)
+  ; BI_const_num (N_to_VAL_i32 ord)
   ; BI_store T_i32 None 2%N 8%N
   ; BI_global_get global_mem_ptr
-  (* ; BI_const_num (nat_to_i32val 12) *)
-  (* ; BI_binop T_i32 (Binop_i BOI_add) *)
   ; BI_global_get global_mem_ptr
   ; BI_store T_i32 None 2%N 12%N
   ; BI_global_get global_mem_ptr
-  ; BI_const_num (nat_to_i32val 8)
+  ; BI_const_num (nat_to_VAL_i32 8)
   ; BI_binop T_i32 (Binop_i BOI_add)
   ] ++ increment_global_mem_ptr 16.
 
-
-Definition apply_carry_operation x y  (ord1 ord2 : nat) (ops relops : list basic_instruction) : list basic_instruction :=
+Definition apply_exact_add_operation (x y : localidx) (addone : bool) : list basic_instruction :=
+    load_local_i64 x ++ load_local_i64 y ++
+    [ BI_binop T_i64 (Binop_i BOI_add) ] ++
+    (if addone then
+       [ BI_const_num 1%Z ; BI_binop T_i64 (Binop_i BOI_add) ]
+     else []) ++
+    bitmask_instrs ++
+    [BI_global_set glob_tmp1 ;BI_global_get glob_tmp1 ] ++
     load_local_i64 x ++
-    load_local_i64 y ++
-    ops ++
-    [ BI_const_num maxuint63
-    ; BI_binop T_i64 (Binop_i BOI_and)
-    ; BI_global_set glob_tmp1
-    ] ++
-    relops ++
-    [ BI_if (BT_valtype (Some (T_num T_i32)))
-        (make_carry ord1 glob_tmp1)
-        (make_carry ord2 glob_tmp1)
+    [ BI_relop T_i64 (Relop_i ((if addone then ROI_le else ROI_lt) SX_U))
+    ; BI_if (BT_valtype (Some (T_num T_i32))) (make_carry C1_ord glob_tmp1) (make_carry C0_ord glob_tmp1)
     ].
 
-(* Assumptions for constructing a prod value:
-   - The 1st argument is stored in global gidx1, 2nd argument in global gidx2
-   - ordinal(pair) = 0 *)
+Definition apply_exact_sub_operation (x y : localidx) (subone : bool) : list basic_instruction :=
+    load_local_i64 x ++ load_local_i64 y ++
+    [ BI_binop T_i64 (Binop_i BOI_sub) ] ++
+    (if subone then
+       [ BI_const_num 1%Z ; BI_binop T_i64 (Binop_i BOI_sub) ]
+     else []) ++
+    bitmask_instrs ++
+    [ BI_global_set glob_tmp1 ] ++
+    load_local_i64 y ++
+    load_local_i64 x ++
+    [ BI_relop T_i64 (Relop_i ((if subone then ROI_lt else ROI_le) SX_U))
+    ; BI_if (BT_valtype (Some (T_num T_i32))) (make_carry C0_ord glob_tmp1) (make_carry C1_ord glob_tmp1)
+    ].
+
+(* Assume 1st element is stored in global gidx1, 2nd element in global gidx2 *)
 Definition make_product (gidx1 gidx2 : N) : list basic_instruction :=
   [ BI_global_get global_mem_ptr
   ; BI_global_get gidx1
   ; BI_store T_i64 None 2%N 0%N
-  (* ; BI_global_get global_mem_ptr *)
-  (* ; BI_const_num (nat_to_i32val 8) *)
-  (* ; BI_binop T_i32 (Binop_i BOI_add) *)
   ; BI_global_get global_mem_ptr
   ; BI_global_get gidx2
   ; BI_store T_i64 None 2%N 8%N
-  (* ; BI_global_get global_mem_ptr *)
-  (* ; BI_const_num (nat_to_i32val 16) *)
-  (* ; BI_binop T_i32 (Binop_i BOI_add) *)
-  (* ; BI_global_set constr_alloc_ptr *)
   ; BI_global_get global_mem_ptr
-  ; BI_const_num (nat_to_i32val 0)
+  ; BI_const_num (N_to_VAL_i32 pair_ord)
   ; BI_store T_i32 None 2%N 16%N
-
-  (* ; BI_global_get global_mem_ptr *)
-  (* ; BI_const_num (nat_to_i32val 20) *)
-  (* ; BI_binop T_i32 (Binop_i BOI_add) *)
   ; BI_global_get global_mem_ptr
   ; BI_global_get global_mem_ptr
   ; BI_store T_i32 None 2%N 20%N
-
   ; BI_global_get global_mem_ptr
-  (* ; BI_const_num (nat_to_i32val 24) *)
-  (* ; BI_binop T_i32 (Binop_i BOI_add) *)
   ; BI_global_get global_mem_ptr
-  ; BI_const_num (nat_to_i32val 8)
+  ; BI_const_num (nat_to_VAL_i32 8)
   ; BI_binop T_i32 (Binop_i BOI_add)
   ; BI_store T_i32 None 2%N 24%N
-
   ; BI_global_get global_mem_ptr
-  ; BI_const_num (nat_to_i32val 16)
+  ; BI_const_num (nat_to_VAL_i32 16)
   ; BI_binop T_i32 (Binop_i BOI_add)
-  (* ; BI_global_get constr_alloc_ptr *)
   ] ++ increment_global_mem_ptr 28.
 
-(* Assumptions about constructor environment for primitive operations that return bools:
-   1. ordinal(true) = 0
-   2. ordinal(false) = 1 *)
 Definition make_boolean_valued_comparison x y relop : list basic_instruction :=
   load_local_i64 x ++            (* Load the arguments onto the stack *)
   load_local_i64 y ++
   [ BI_relop T_i64 (Relop_i relop)
   ; BI_if (BT_valtype (Some (T_num T_i32)))
-      [ BI_const_num (nat_to_i32val 1) ] (* 2 * ordinal(true) + 1 *)
-      [ BI_const_num (nat_to_i32val 3) ] (* 2 * ordinal(false) + 1 *)
+      [ BI_const_num (N_to_VAL_i32 (2 * true_ord + 1)) ]
+      [ BI_const_num (N_to_VAL_i32 (2 * false_ord + 1)) ]
   ].
 
-Definition translate_primitive_binary_op op_name x y : error (list basic_instruction) :=
-  if Kername.eqb op_name primInt63Add then
-    Ret (apply_binop_and_store_i64 [ BI_binop T_i64 (Binop_i BOI_add) ; BI_const_num maxuint63 ; BI_binop T_i64 (Binop_i BOI_and) ] x y)
-  else if Kername.eqb op_name primInt63Sub then
-    Ret (apply_binop_and_store_i64 [ BI_binop T_i64 (Binop_i BOI_sub) ; BI_const_num maxuint63 ; BI_binop T_i64 (Binop_i BOI_and) ] x y)
-  else if Kername.eqb op_name primInt63Mul then
-    Ret (apply_binop_and_store_i64 [ BI_binop T_i64 (Binop_i BOI_mul) ; BI_const_num maxuint63 ; BI_binop T_i64 (Binop_i BOI_and) ] x y)
-  else if Kername.eqb op_name primInt63Div then
-    Ret (BI_global_get global_mem_ptr ::
-         load_local_i64 y ++
-         [ BI_testop T_i64 TO_eqz
-         ; BI_if (BT_valtype (Some (T_num T_i64)))
-             [ BI_const_num (nat_to_i64val 0) ]
-             (load_local_i64 x ++ load_local_i64 y ++ [ BI_binop T_i64 (Binop_i (BOI_div SX_U)) ])
-         ; BI_store T_i64 None 2%N 0%N
-         ; BI_global_get global_mem_ptr
-         ] ++ increment_global_mem_ptr 8)
-  else if Kername.eqb op_name primInt63Mod then
-    Ret(BI_global_get global_mem_ptr ::
-        load_local_i64 y ++
-        [ BI_testop T_i64 TO_eqz
-        ; BI_if (BT_valtype (Some (T_num T_i64)))
-            (load_local_i64 x)
-            (load_local_i64 x ++ load_local_i64 y ++ [ BI_binop T_i64 (Binop_i (BOI_rem SX_U)) ])
-        ; BI_store T_i64 None 2%N 0%N
-        ; BI_global_get global_mem_ptr
-        ] ++ increment_global_mem_ptr 8)
-  else if Kername.eqb op_name primInt63Land then
-    Ret (apply_binop_and_store_i64 [ BI_binop T_i64 (Binop_i BOI_and) ] x y)
-  else if Kername.eqb op_name primInt63Lor then
-    Ret (apply_binop_and_store_i64 [ BI_binop T_i64 (Binop_i BOI_or) ] x y)
-  else if Kername.eqb op_name primInt63Lxor then
-    Ret (apply_binop_and_store_i64 [ BI_binop T_i64 (Binop_i BOI_xor) ] x y)
-  else if Kername.eqb op_name primInt63Lsl then
-    Ret (BI_global_get global_mem_ptr ::
-         load_local_i64 y ++
-         [ BI_const_num (nat_to_i64val 63)
-         ; BI_relop T_i64 (Relop_i (ROI_lt SX_U))
-         ; BI_if (BT_valtype (Some (T_num T_i64)))
-             (load_local_i64 x ++
-              load_local_i64 y ++
-              [ BI_binop T_i64 (Binop_i BOI_shl) ; BI_const_num maxuint63 ; BI_binop T_i64 (Binop_i BOI_and) ])
-             [ BI_const_num (nat_to_i64val 0) ]
-         ; BI_store T_i64 None 2%N 0%N
-         ; BI_global_get global_mem_ptr
-         ] ++ increment_global_mem_ptr 8)
 
-  else if Kername.eqb op_name primInt63Lsr then
-    Ret (BI_global_get global_mem_ptr ::
-         load_local_i64 y ++
-         [ BI_const_num (nat_to_i64val 63)
-         ; BI_relop T_i64 (Relop_i (ROI_lt SX_U))
-         ; BI_if (BT_valtype (Some (T_num T_i64)))
-             (load_local_i64 x ++ load_local_i64 y ++ [ BI_binop T_i64 (Binop_i (BOI_shr SX_U)) ])
-             [ BI_const_num (nat_to_i64val 0) ]
-         ; BI_store T_i64 None 2%N 0%N
-         ; BI_global_get global_mem_ptr
-         ] ++ increment_global_mem_ptr 8)
+Definition compare_instrs x y : list basic_instruction :=
+  [ BI_local_get x
+    ; BI_load T_i64 None 2%N 0%N
+    ; BI_local_get y
+    ; BI_load T_i64 None 2%N 0%N
+    ; BI_relop T_i64 (Relop_i (ROI_lt SX_U))
+    ; BI_if (BT_valtype (Some (T_num T_i32)))
+        [ BI_const_num (N_to_VAL_i32 (2 * Lt_ord + 1)) ]
+        (load_local_i64 x ++
+           load_local_i64 y ++
+           [ BI_relop T_i64 (Relop_i ROI_eq)
+           ; BI_if (BT_valtype (Some (T_num T_i32)))
+               [ BI_const_num (N_to_VAL_i32 (2 * Eq_ord + 1)) ]
+               [ BI_const_num (N_to_VAL_i32 (2 * Gt_ord + 1)) ]
+           ])
+  ].
 
-  else if Kername.eqb op_name primInt63Eqb then
-    Ret (make_boolean_valued_comparison x y ROI_eq)
+Definition div_instrs (x y : localidx) : list basic_instruction :=
+  BI_global_get global_mem_ptr ::
+    load_local_i64 y ++
+    [ BI_testop T_i64 TO_eqz
+    ; BI_if (BT_valtype (Some (T_num T_i64)))
+        [ BI_const_num 0%Z ]
+        (load_local_i64 x ++ load_local_i64 y ++ [ BI_binop T_i64 (Binop_i (BOI_div SX_U)) ])
+    ; BI_store T_i64 None 2%N 0%N
+    ; BI_global_get global_mem_ptr
+    ] ++ increment_global_mem_ptr 8.
 
-  else if Kername.eqb op_name primInt63Ltb then
-    Ret (make_boolean_valued_comparison x y (ROI_lt SX_U))
 
-  else if Kername.eqb op_name primInt63Leb then
-    Ret (make_boolean_valued_comparison x y (ROI_le SX_U))
+Definition mod_instrs (x y : localidx) : list basic_instruction :=
+  BI_global_get global_mem_ptr ::
+    load_local_i64 y ++
+    [ BI_testop T_i64 TO_eqz
+    ; BI_if (BT_valtype (Some (T_num T_i64)))
+        (load_local_i64 x)
+        (load_local_i64 x ++ load_local_i64 y ++ [ BI_binop T_i64 (Binop_i (BOI_rem SX_U)) ])
+    ; BI_store T_i64 None 2%N 0%N
+    ; BI_global_get global_mem_ptr
+    ] ++ increment_global_mem_ptr 8.
 
-  (* Assumptions about constructor environment for compare:
-       1. ordinal(Eq) = 0
-       2. ordinal(Lt) = 1
-       3. ordinal(Gt) = 2 *)
-  else if Kername.eqb op_name primInt63Compare then
-    Ret ([ BI_local_get x
-         ; BI_load T_i64 None 2%N 0%N
-         ; BI_local_get y
-         ; BI_load T_i64 None 2%N 0%N
-         ; BI_relop T_i64 (Relop_i (ROI_lt SX_U))
-         ; BI_if (BT_valtype (Some (T_num T_i32)))
-             [ BI_const_num (nat_to_i32val 3) ] (* 2 * ordinal(Lt) + 1 *)
-             (load_local_i64 x ++
-              load_local_i64 y ++
-              [ BI_relop T_i64 (Relop_i ROI_eq)
-              ; BI_if (BT_valtype (Some (T_num T_i32)))
-                  [ BI_const_num (nat_to_i32val 1) ] (* 2 * ordinal(Eq) + 1 *)
-                  [ BI_const_num (nat_to_i32val 5) ] (* 2 * ordinal(Gt) + 1*)
-              ])
-         ])
+Definition shift_instrs (x y : localidx) shiftop (mask : bool) : list basic_instruction :=
+  BI_global_get global_mem_ptr ::
+    load_local_i64 y ++
+    [ BI_const_num 63%Z
+    ; BI_relop T_i64 (Relop_i (ROI_lt SX_U))
+    ; BI_if (BT_valtype (Some (T_num T_i64)))
+        (load_local_i64 x ++
+           load_local_i64 y ++
+           BI_binop T_i64 (Binop_i shiftop) ::
+           (if mask then bitmask_instrs else []))
+        [ BI_const_num 0%Z ]
+    ; BI_store T_i64 None 2%N 0%N
+    ; BI_global_get global_mem_ptr
+    ] ++ increment_global_mem_ptr 8.
 
-       (* Assumptions for constructing a carry value:
-          - The argument is stored in global with index gidx
-          - ordinal(C0) = 0
-          - ordinal(C1) = 1 *)
-  else if Kername.eqb op_name primInt63Addc then
-    Ret (apply_carry_operation x y 1 0
-           [ BI_binop T_i64 (Binop_i BOI_add) ]
-           ([ BI_global_get glob_tmp1 ] ++
-              load_local_i64 x ++
-              [ BI_relop T_i64 (Relop_i (ROI_lt SX_U))]))
+Definition mulc_instrs (x y : localidx) : list basic_instruction :=
+  load_local_i64 x ++
+    [ BI_const_num 62%Z ; BI_binop T_i64 (Binop_i (BOI_shr SX_U)) ; BI_testop T_i64 TO_eqz ] ++
+    load_local_i64 y ++
+    [ BI_const_num 62%Z ; BI_binop T_i64 (Binop_i (BOI_shr SX_U)) ; BI_testop T_i64 TO_eqz ] ++
+    [ BI_binop T_i32 (Binop_i BOI_or)
+    ; BI_if (BT_valtype None)
+        (load_local_i64 y ++ [ BI_global_set glob_tmp3 ])
+        (load_local_i64 y ++
+             [ BI_const_num (VAL_int64 (Wasm_int.Int64.repr 4611686018427387904%Z))
+             ; BI_binop T_i64 (Binop_i BOI_xor)
+             ; BI_global_set glob_tmp3
+             ])
+    ] ++
+    (* glob_tmp1 <- let hx = x >> 31 *)
+    load_local_i64 x ++
+    [ BI_const_num 31%Z ; BI_binop T_i64 (Binop_i (BOI_shr SX_U)) ; BI_global_set glob_tmp1 ] ++
+    (* glob_tmp2 <- let lx = x & ((1 << 31) - 1) *)
+    load_local_i64 x ++
+    [ BI_const_num maxuint31 ; BI_binop T_i64 (Binop_i BOI_and) ; BI_global_set glob_tmp2 ] ++
+    (* glob_tmp4 <- let hy =  y >> 31 *)
+    [ BI_global_get glob_tmp3 ; BI_const_num 31%Z ; BI_binop T_i64 (Binop_i (BOI_shr SX_U)) ; BI_global_set glob_tmp4 ] ++
+    (* glob_tmp3 <- let ly = y & ((1 << 31) - 1) *)
+    [ BI_global_get glob_tmp3 ; BI_const_num maxuint31 ; BI_binop T_i64 (Binop_i BOI_and) ; BI_global_set glob_tmp3 ] ++
+    [ BI_global_get glob_tmp1 ; BI_global_get glob_tmp4 ; BI_binop T_i64 (Binop_i BOI_mul) ] ++
+    [ BI_global_get glob_tmp1 ; BI_global_get glob_tmp3 ; BI_binop T_i64 (Binop_i BOI_mul) ] ++
+    [ BI_global_get glob_tmp2 ; BI_global_get glob_tmp4 ; BI_binop T_i64 (Binop_i BOI_mul) ] ++
+    [ BI_global_get glob_tmp2 ; BI_global_get glob_tmp3 ; BI_binop T_i64 (Binop_i BOI_mul) ] ++
+    (* glob_tmp4 <- let lxy = lx * ly
+       glob_tmp3 <- let lxhy = lx * hy
+       glob_tmp2 <- let hxly = hx * ly
+       glob_tmp1 <- let hxy  = hx * hy *)
+    [ BI_global_set glob_tmp4
+    ; BI_global_set glob_tmp3
+    ; BI_global_set glob_tmp2
+    ; BI_global_set glob_tmp1
+    ]  ++
+    (* glob_tmp4 <- let l = lxy | (hxy << 62) = glob_tmp4 | (glob_tmp1 << 62) *)
+    [ BI_global_get glob_tmp4
+    ; BI_global_get glob_tmp1
+    ; BI_const_num 62%Z
+    ; BI_binop T_i64 (Binop_i BOI_shl)
+    ; BI_const_num maxuint63
+    ; BI_binop T_i64 (Binop_i BOI_and)
+    ; BI_binop T_i64 (Binop_i BOI_or)
+    ; BI_global_set glob_tmp4
+    ] ++
+    (* glob_tmp1 <- let h = hxy >> 1 = glob_tmp1 >> 1 *)
+    [ BI_global_get glob_tmp1
+    ; BI_const_num 1%Z
+    ; BI_binop T_i64 (Binop_i (BOI_shr SX_U))
+    ; BI_global_set glob_tmp1
+    ] ++
+    (* glob_tmp3 <- let hl = hxly + lxhy = glob_tmp2 + glob_tmp3 *)
+    [ BI_global_get glob_tmp2
+    ; BI_global_get glob_tmp3
+    ; BI_binop T_i64 (Binop_i BOI_add)
+    ; BI_const_num maxuint63
+    ; BI_binop T_i64 (Binop_i BOI_and)
+    ; BI_global_set glob_tmp3
+    ] ++
+    (* glob_tmp1 <- let h = if hl < hxly then h + (1 << 31) else h *)
+    [ BI_global_get glob_tmp3
+    ; BI_global_get glob_tmp2
+    ; BI_relop T_i64 (Relop_i (ROI_lt SX_U))
+    ; BI_if (BT_valtype None)
+        [ BI_global_get glob_tmp1
+        ; BI_const_num (VAL_int64 (Wasm_int.Int64.repr 2147483648%Z))
+        ; BI_binop T_i64 (Binop_i BOI_add)
+        ; BI_global_set glob_tmp1
+        ]
+        [ ]
+    ] ++
+    (* glob_tmp2 <- let hl' = hl << 31 *)
+    [ BI_global_get glob_tmp3
+    ; BI_const_num 31%Z
+    ; BI_binop T_i64 (Binop_i BOI_shl)
+    ; BI_const_num maxuint63
+    ; BI_binop T_i64 (Binop_i BOI_and)
+    ; BI_global_set glob_tmp2
+    ] ++
+    (* glob_tmp4 <- let l = l + hl' *)
+    [ BI_global_get glob_tmp4
+    ; BI_global_get glob_tmp2
+    ; BI_binop T_i64 (Binop_i BOI_add)
+    ; BI_const_num maxuint63
+    ; BI_binop T_i64 (Binop_i BOI_and)
+    ; BI_global_set glob_tmp4
+    ] ++
+    (* glob_tmp1 <- let h = if l < hl' then h + 1 else h *)
+    [ BI_global_get glob_tmp4
+    ; BI_global_get glob_tmp2
+    ; BI_relop T_i64 (Relop_i (ROI_lt SX_U))
+    ; BI_if (BT_valtype None)
+        [ BI_global_get glob_tmp1
+        ; BI_const_num 1%Z
+        ; BI_binop T_i64 (Binop_i BOI_add)
+        ; BI_global_set glob_tmp1
+        ]
+        [ ]
+    ] ++
+    (* glob_tmp1 <- let h = h + (hl >> 32) *)
+    [ BI_global_get glob_tmp1
+    ; BI_global_get glob_tmp3
+    ; BI_const_num 32%Z
+    ; BI_binop T_i64 (Binop_i (BOI_shr SX_U))
+    ; BI_binop T_i64 (Binop_i BOI_add)
+    ; BI_const_num maxuint63
+    ; BI_binop T_i64 (Binop_i BOI_and)
+    ; BI_global_set glob_tmp1
+    ] ++
+    load_local_i64 x ++
+    [ BI_const_num 62%Z
+    ; BI_binop T_i64 (Binop_i (BOI_shr SX_U))
+    ; BI_testop T_i64 TO_eqz
+    ] ++
+    load_local_i64 y ++
+    [ BI_const_num 62%Z
+    ; BI_binop T_i64 (Binop_i (BOI_shr SX_U))
+    ; BI_testop T_i64 TO_eqz
+    ; BI_binop T_i32 (Binop_i BOI_or)
+    ; BI_if (BT_valtype None)
+        [ ]
+        [ (* glob_tmp2 <- let l' := l + (x << 62) *)
+        BI_global_get glob_tmp4
+        ; BI_local_get x
+        ; BI_load T_i64 None 2%N 0%N
+        ; BI_const_num 62%Z
+        ; BI_binop T_i64 (Binop_i BOI_shl)
+        ; BI_binop T_i64 (Binop_i BOI_add)
+        ; BI_const_num maxuint63
+        ; BI_binop T_i64 (Binop_i BOI_and)
+        ; BI_global_set glob_tmp2
+        (* glob_tmp1 <- let h := if l' < l then h + 1 else h *)
+        ; BI_global_get glob_tmp2
+        ; BI_global_get glob_tmp4
+        ; BI_relop T_i64 (Relop_i (ROI_lt SX_U))
+        ; BI_if (BT_valtype None)
+            [ BI_global_get glob_tmp1
+            ; BI_const_num 1%Z
+            ; BI_binop T_i64 (Binop_i BOI_add)
+            ; BI_global_set glob_tmp1
+            ]
+            [ ]
+        (* return (h + (x >> 1), l') *)
+        ; BI_global_get glob_tmp1
+        ; BI_local_get x
+        ; BI_load T_i64 None 2%N 0%N
+        ; BI_const_num 1%Z
+        ; BI_binop T_i64 (Binop_i (BOI_shr SX_U))
+        ; BI_binop T_i64 (Binop_i BOI_add)
+        ; BI_const_num maxuint63
+        ; BI_binop T_i64 (Binop_i BOI_and)
+        ; BI_global_set glob_tmp1
+        ; BI_global_get glob_tmp2
+        ; BI_global_set glob_tmp4
+        ]
+    ] ++ make_product glob_tmp1 glob_tmp4.
 
-  else if Kername.eqb op_name primInt63Addcarryc then
-    Ret (apply_carry_operation x y 1 0
-           [ BI_binop T_i64 (Binop_i BOI_add)
-             ; BI_const_num (nat_to_i64val 1)
-             ; BI_binop T_i64 (Binop_i BOI_add) ]
-           ([ BI_global_get glob_tmp1 ] ++
-              load_local_i64 x ++
-              [ BI_relop T_i64 (Relop_i (ROI_le SX_U))]))
+Definition diveucl_instrs (x y : localidx) : list basic_instruction :=
+  [ BI_local_get x
+  ; BI_load T_i64 None 2%N 0%N
+  ; BI_testop T_i64 TO_eqz
+  ; BI_if (BT_valtype None)
+      [ BI_const_num (VAL_int64 (Z_to_i64 0))
+      ; BI_global_set glob_tmp1
+      ; BI_const_num 0%Z
+      ; BI_global_set glob_tmp2
+      ]
+      [ BI_local_get y
+      ; BI_load T_i64 None 2%N 0%N
+      ; BI_testop T_i64 TO_eqz
+      ; BI_if (BT_valtype None)
+          [ BI_const_num (VAL_int64 (Z_to_i64 0))
+          ; BI_global_set glob_tmp1
+          ; BI_local_get x
+          ; BI_load T_i64 None 2%N 0%N
+          ; BI_global_set glob_tmp2
+          ]
+          (load_local_i64 x ++
+             load_local_i64 y ++
+             [ BI_binop T_i64 (Binop_i (BOI_div SX_U)) ; BI_global_set glob_tmp1 ] ++
+             load_local_i64 x ++
+             load_local_i64 y ++
+             [ BI_binop T_i64 (Binop_i (BOI_rem SX_U)) ; BI_global_set glob_tmp2 ])
+      ]
+  ] ++ make_product glob_tmp1 glob_tmp2.
 
-  else if Kername.eqb op_name primInt63Subc then
-    Ret (apply_carry_operation x y 0 1
-           [ BI_binop T_i64 (Binop_i BOI_sub) ]
-           (load_local_i64 y ++
-              load_local_i64 x ++
-              [ BI_relop T_i64 (Relop_i (ROI_le SX_U))]))
+Definition translate_primitive_binary_op op (x y : localidx) : error (list basic_instruction) :=
+  match op with
+  | PrimInt63add       => Ret (apply_binop_and_store_i64 BOI_add x y true)
+  | PrimInt63sub       => Ret (apply_binop_and_store_i64 BOI_sub x y true)
+  | PrimInt63mul       => Ret (apply_binop_and_store_i64 BOI_mul x y true)
+  | PrimInt63div       => Ret (div_instrs x y)
+  | PrimInt63mod       => Ret (mod_instrs x y)
+  | PrimInt63lsl       => Ret (shift_instrs x y BOI_shl true)
+  | PrimInt63lsr       => Ret (shift_instrs x y (BOI_shr SX_U) false)
+  | PrimInt63land      => Ret (apply_binop_and_store_i64 BOI_and x y false)
+  | PrimInt63lor       => Ret (apply_binop_and_store_i64 BOI_or x y false)
+  | PrimInt63lxor      => Ret (apply_binop_and_store_i64 BOI_xor x y false)
+  | PrimInt63eqb       => Ret (make_boolean_valued_comparison x y ROI_eq)
+  | PrimInt63ltb       => Ret (make_boolean_valued_comparison x y (ROI_lt SX_U))
+  | PrimInt63leb       => Ret (make_boolean_valued_comparison x y (ROI_le SX_U))
+  | PrimInt63compare   => Ret (compare_instrs x y)
+  | PrimInt63addc      => Ret (apply_exact_add_operation x y false)
+  | PrimInt63addcarryc => Ret (apply_exact_add_operation x y true)
+  | PrimInt63subc      => Ret (apply_exact_sub_operation x y false)
+  | PrimInt63subcarryc => Ret (apply_exact_sub_operation x y true)
+  | PrimInt63mulc      => Ret (mulc_instrs x y)
+  | PrimInt63diveucl   => Ret (diveucl_instrs x y)
+  | _ => Err "Unknown primitive binary operator"
+  end.
 
-  else if Kername.eqb op_name primInt63Subcarryc then
-    Ret (apply_carry_operation x y 0 1
-           [ BI_binop T_i64 (Binop_i BOI_sub)
-           ; BI_const_num (nat_to_i64val 1)
-           ; BI_binop T_i64 (Binop_i BOI_sub) ]
-           (load_local_i64 y ++
-              load_local_i64 x ++
-              [ BI_relop T_i64 (Relop_i (ROI_lt SX_U))]))
+(* head0 x computes the leading number of zeros in x
+   OBS: need to subtract 1 since we're dealing with 63-bit integers *)
+Definition head0_instrs (x : localidx) : list basic_instruction :=
+  BI_global_get global_mem_ptr ::
+    load_local_i64 x ++
+    [ BI_unop T_i64 (Unop_i UOI_clz)
+    ; BI_const_num 1%Z
+    ; BI_binop T_i64 (Binop_i BOI_sub)
+    ; BI_store T_i64 None 2%N 0%N
+    ; BI_global_get global_mem_ptr
+    ] ++ increment_global_mem_ptr 8.
 
-  else if Kername.eqb op_name primInt63Mulc then
-    Ret (load_local_i64 x ++
-         [ BI_const_num (nat_to_i64val 62) ; BI_binop T_i64 (Binop_i (BOI_shr SX_U)) ; BI_testop T_i64 TO_eqz ] ++
-         load_local_i64 y ++
-         [ BI_const_num (nat_to_i64val 62) ; BI_binop T_i64 (Binop_i (BOI_shr SX_U)) ; BI_testop T_i64 TO_eqz ] ++
-         [ BI_binop T_i32 (Binop_i BOI_or)
-         ; BI_if (BT_valtype None)
-             (load_local_i64 y ++ [ BI_global_set glob_tmp3 ])
-             (load_local_i64 y ++
-              [ BI_const_num (VAL_int64 (Wasm_int.Int64.repr 4611686018427387904%Z))
-              ; BI_binop T_i64 (Binop_i BOI_xor)
-              ; BI_global_set glob_tmp3
-              ])
-         ] ++
-         (* glob_tmp1 <- let hx = x >> 31 *)
-         load_local_i64 x ++
-         [ BI_const_num (nat_to_i64val 31) ; BI_binop T_i64 (Binop_i (BOI_shr SX_U)) ; BI_global_set glob_tmp1 ] ++
-         (* glob_tmp2 <- let lx = x & ((1 << 31) - 1) *)
-         load_local_i64 x ++
-         [ BI_const_num maxuint31 ; BI_binop T_i64 (Binop_i BOI_and) ; BI_global_set glob_tmp2 ] ++
-         (* glob_tmp4 <- let hy =  y >> 31 *)
-         [ BI_global_get glob_tmp3 ; BI_const_num (nat_to_i64val 31) ; BI_binop T_i64 (Binop_i (BOI_shr SX_U)) ; BI_global_set glob_tmp4 ] ++
-         (* glob_tmp3 <- let ly = y & ((1 << 31) - 1) *)
-         [ BI_global_get glob_tmp3 ; BI_const_num maxuint31 ; BI_binop T_i64 (Binop_i BOI_and) ; BI_global_set glob_tmp3 ] ++
-         [ BI_global_get glob_tmp1 ; BI_global_get glob_tmp4 ; BI_binop T_i64 (Binop_i BOI_mul) ] ++
-         [ BI_global_get glob_tmp1 ; BI_global_get glob_tmp3 ; BI_binop T_i64 (Binop_i BOI_mul) ] ++
-         [ BI_global_get glob_tmp2 ; BI_global_get glob_tmp4 ; BI_binop T_i64 (Binop_i BOI_mul) ] ++
-         [ BI_global_get glob_tmp2 ; BI_global_get glob_tmp3 ; BI_binop T_i64 (Binop_i BOI_mul) ] ++
-         (* glob_tmp4 <- let lxy = lx * ly
-            glob_tmp3 <- let lxhy = lx * hy
-            glob_tmp2 <- let hxly = hx * ly
-            glob_tmp1 <- let hxy  = hx * hy *)
-         [ BI_global_set glob_tmp4
-         ; BI_global_set glob_tmp3
-         ; BI_global_set glob_tmp2
-         ; BI_global_set glob_tmp1
-         ]  ++
-         (* glob_tmp4 <- let l = lxy | (hxy << 62) = glob_tmp4 | (glob_tmp1 << 62) *)
-         [ BI_global_get glob_tmp4
-         ; BI_global_get glob_tmp1
-         ; BI_const_num (nat_to_i64val 62)
-         ; BI_binop T_i64 (Binop_i BOI_shl)
-         ; BI_const_num maxuint63
-         ; BI_binop T_i64 (Binop_i BOI_and)
-         ; BI_binop T_i64 (Binop_i BOI_or)
-         ; BI_global_set glob_tmp4
-         ] ++
-         (* glob_tmp1 <- let h = hxy >> 1 = glob_tmp1 >> 1 *)
-         [ BI_global_get glob_tmp1
-         ; BI_const_num (nat_to_i64val 1)
-         ; BI_binop T_i64 (Binop_i (BOI_shr SX_U))
-         ; BI_global_set glob_tmp1
-         ] ++
-         (* glob_tmp3 <- let hl = hxly + lxhy = glob_tmp2 + glob_tmp3 *)
-         [ BI_global_get glob_tmp2
-         ; BI_global_get glob_tmp3
-         ; BI_binop T_i64 (Binop_i BOI_add)
-         ; BI_const_num maxuint63
-         ; BI_binop T_i64 (Binop_i BOI_and)
-         ; BI_global_set glob_tmp3
-         ] ++
-         (* glob_tmp1 <- let h = if hl < hxly then h + (1 << 31) else h *)
-         [ BI_global_get glob_tmp3
-         ; BI_global_get glob_tmp2
-         ; BI_relop T_i64 (Relop_i (ROI_lt SX_U))
-         ; BI_if (BT_valtype None)
-             [ BI_global_get glob_tmp1
-             ; BI_const_num (VAL_int64 (Wasm_int.Int64.repr 2147483648%Z))
-             ; BI_binop T_i64 (Binop_i BOI_add)
-             ; BI_global_set glob_tmp1
-             ]
-             [ ]
-         ] ++
-         (* glob_tmp2 <- let hl' = hl << 31 *)
-         [ BI_global_get glob_tmp3
-         ; BI_const_num (nat_to_i64val 31)
-         ; BI_binop T_i64 (Binop_i BOI_shl)
-         ; BI_const_num maxuint63
-         ; BI_binop T_i64 (Binop_i BOI_and)
-         ; BI_global_set glob_tmp2
-         ] ++
-         (* glob_tmp4 <- let l = l + hl' *)
-         [ BI_global_get glob_tmp4
-         ; BI_global_get glob_tmp2
-         ; BI_binop T_i64 (Binop_i BOI_add)
-         ; BI_const_num maxuint63
-         ; BI_binop T_i64 (Binop_i BOI_and)
-         ; BI_global_set glob_tmp4
-         ] ++
-         (* glob_tmp1 <- let h = if l < hl' then h + 1 else h *)
-         [ BI_global_get glob_tmp4
-         ; BI_global_get glob_tmp2
-         ; BI_relop T_i64 (Relop_i (ROI_lt SX_U))
-         ; BI_if (BT_valtype None)
-             [ BI_global_get glob_tmp1
-             ; BI_const_num (nat_to_i64val 1)
-             ; BI_binop T_i64 (Binop_i BOI_add)
-             ; BI_global_set glob_tmp1
-             ]
-             [ ]
-         ] ++
-         (* glob_tmp1 <- let h = h + (hl >> 32) *)
-         [ BI_global_get glob_tmp1
-         ; BI_global_get glob_tmp3
-         ; BI_const_num (nat_to_i64val 32)
-         ; BI_binop T_i64 (Binop_i (BOI_shr SX_U))
-         ; BI_binop T_i64 (Binop_i BOI_add)
-         ; BI_const_num maxuint63
-         ; BI_binop T_i64 (Binop_i BOI_and)
-         ; BI_global_set glob_tmp1
-         ] ++
-         load_local_i64 x ++
-         [ BI_const_num (nat_to_i64val 62)
-         ; BI_binop T_i64 (Binop_i (BOI_shr SX_U))
-         ; BI_testop T_i64 TO_eqz
-         ] ++
-         load_local_i64 y ++
-         [ BI_const_num (nat_to_i64val 62)
-         ; BI_binop T_i64 (Binop_i (BOI_shr SX_U))
-         ; BI_testop T_i64 TO_eqz
-         ; BI_binop T_i32 (Binop_i BOI_or)
-         ; BI_if (BT_valtype None)
-             [ ]
-             [ (* glob_tmp2 <- let l' := l + (x << 62) *)
-             BI_global_get glob_tmp4
-             ; BI_local_get x
-             ; BI_load T_i64 None 2%N 0%N
-             ; BI_const_num (nat_to_i64val 62)
-             ; BI_binop T_i64 (Binop_i BOI_shl)
-             ; BI_binop T_i64 (Binop_i BOI_add)
-             ; BI_const_num maxuint63
-             ; BI_binop T_i64 (Binop_i BOI_and)
-             ; BI_global_set glob_tmp2
-             (* glob_tmp1 <- let h := if l' < l then h + 1 else h *)
-             ; BI_global_get glob_tmp2
-             ; BI_global_get glob_tmp4
-             ; BI_relop T_i64 (Relop_i (ROI_lt SX_U))
-             ; BI_if (BT_valtype None)
-                 [ BI_global_get glob_tmp1
-                 ; BI_const_num (nat_to_i64val 1)
-                 ; BI_binop T_i64 (Binop_i BOI_add)
-                 ; BI_global_set glob_tmp1
-                 ]
-                 [ ]
-             (* return (h + (x >> 1), l') *)
-             ; BI_global_get glob_tmp1
-             ; BI_local_get x
-             ; BI_load T_i64 None 2%N 0%N
-             ; BI_const_num (nat_to_i64val 1)
-             ; BI_binop T_i64 (Binop_i (BOI_shr SX_U))
-             ; BI_binop T_i64 (Binop_i BOI_add)
-             ; BI_const_num maxuint63
-             ; BI_binop T_i64 (Binop_i BOI_and)
-             ; BI_global_set glob_tmp1
-             ; BI_global_get glob_tmp2
-             ; BI_global_set glob_tmp4
-             ]
-         ] ++ make_product glob_tmp1 glob_tmp4)
+(* tail0 x computes the trailing number of zeros in x
+   OBS: if x is 0, then result is 63 (can't just use wasm ctz op) ) *)
+Definition tail0_instrs (x : localidx) : list basic_instruction :=
+  BI_global_get global_mem_ptr ::
+    load_local_i64 x ++
+    [ BI_testop T_i64 TO_eqz
+    ; BI_if (BT_valtype (Some (T_num T_i64)))
+        [ BI_const_num 63%Z ]
+        (load_local_i64 x ++ [ BI_unop T_i64 (Unop_i UOI_ctz) ])
+    ; BI_store T_i64 None 2%N 0%N
+    ; BI_global_get global_mem_ptr
+    ] ++ increment_global_mem_ptr 8.
 
-  else if Kername.eqb op_name primInt63Diveucl then
-    Ret ([ BI_local_get x
-         ; BI_load T_i64 None 2%N 0%N
-         ; BI_testop T_i64 TO_eqz
-         ; BI_if (BT_valtype None)
-             [ BI_const_num (nat_to_i64val 0)
-             ; BI_global_set glob_tmp1
-             ; BI_const_num (nat_to_i64val 0)
-             ; BI_global_set glob_tmp2
-             ]
-             [ BI_local_get y
-             ; BI_load T_i64 None 2%N 0%N
-             ; BI_testop T_i64 TO_eqz
-             ; BI_if (BT_valtype None)
-                 [ BI_const_num (nat_to_i64val 0)
-                 ; BI_global_set glob_tmp1
-                 ; BI_local_get x
-                 ; BI_load T_i64 None 2%N 0%N
-                 ; BI_global_set glob_tmp2
-                 ]
-                 (load_local_i64 x ++
-                  load_local_i64 y ++
-                  [ BI_binop T_i64 (Binop_i (BOI_div SX_U)) ; BI_global_set glob_tmp1 ] ++
-                  load_local_i64 x ++
-                  load_local_i64 y ++
-                  [ BI_binop T_i64 (Binop_i (BOI_rem SX_U)) ; BI_global_set glob_tmp2 ])
-             ]
-         ] ++ make_product glob_tmp1 glob_tmp2)
-  else
-    Err ("Unknown primitive arithmetic operator: " ++ (Kernames.string_of_kername op_name))%bs.
+Definition translate_primitive_unary_op op (x : localidx) : error (list basic_instruction) :=
+  match op with
+  | PrimInt63head0 => Ret (head0_instrs x)
+  | PrimInt63tail0 => Ret (tail0_instrs x)
+  | _ => Err "Unknown primitive unary operator"
+  end.
 
-Definition translate_primitive_unary_op op_name x : error (list basic_instruction) :=
-  if Kername.eqb op_name primInt63Head0 then
-    (* head0 x computes the leading number of zeros in x
-           OBS: need to subtract 1 since we're dealing with 63-bit integers *)
-    Ret (BI_global_get global_mem_ptr ::
-         load_local_i64 x ++
-         [ BI_unop T_i64 (Unop_i UOI_clz)
-         ; BI_const_num (nat_to_i64val 1)
-         ; BI_binop T_i64 (Binop_i BOI_sub)
-         ; BI_store T_i64 None 2%N 0%N
-         ; BI_global_get global_mem_ptr
-         ] ++ increment_global_mem_ptr 8)
-
-  else if Kername.eqb op_name primInt63Tail0 then
-    (* tail0 x computes the trailing number of zeros in x
-           OBS: if x is 0, then result is 63 (can't just use wasm ctz op) ) *)
-    Ret (BI_global_get global_mem_ptr ::
-         load_local_i64 x ++
-         [ BI_testop T_i64 TO_eqz
-         ; BI_if (BT_valtype (Some (T_num T_i64)))
-             [ BI_const_num (nat_to_i64val 63) ]
-             (load_local_i64 x ++ [ BI_unop T_i64 (Unop_i UOI_ctz) ])
-         ; BI_store T_i64 None 2%N 0%N
-         ; BI_global_get global_mem_ptr
-         ] ++ increment_global_mem_ptr 8)
-  else
-    Err ("Unknown primitive unary operator: " ++ (Kernames.string_of_kername op_name))%bs.
-
-Definition div21_loop_body :=
+Definition diveucl_21_loop_body :=
   [ BI_global_get glob_tmp1
-  ; BI_const_num (nat_to_i64val 1)
+  ; BI_const_num 1%Z
   ; BI_binop T_i64 (Binop_i BOI_shl)
   ; BI_global_get glob_tmp2
-  ; BI_const_num (nat_to_i64val 62)
+  ; BI_const_num 62%Z
   ; BI_binop T_i64 (Binop_i (BOI_shr SX_U))
   ; BI_binop T_i64 (Binop_i BOI_or)
   ; BI_global_set glob_tmp1
 
   ; BI_global_get glob_tmp2
-  ; BI_const_num (nat_to_i64val 1)
+  ; BI_const_num 1%Z
   ; BI_binop T_i64 (Binop_i BOI_shl)
   ; BI_const_num maxuint63
   ; BI_binop T_i64 (Binop_i (BOI_rem SX_U))
   ; BI_global_set glob_tmp2
 
   ; BI_global_get glob_tmp3
-  ; BI_const_num (nat_to_i64val 1)
+  ; BI_const_num 1%Z
   ; BI_binop T_i64 (Binop_i BOI_shl)
   ; BI_const_num maxuint63
   ; BI_binop T_i64 (Binop_i BOI_and)
@@ -546,7 +551,7 @@ Definition div21_loop_body :=
   ; BI_relop T_i64 (Relop_i (ROI_ge SX_U))
   ; BI_if (BT_valtype None)
       [ BI_global_get glob_tmp3
-      ; BI_const_num (nat_to_i64val 1)
+      ; BI_const_num 1%Z
       ; BI_binop T_i64 (Binop_i BOI_or)
       ; BI_global_set glob_tmp3
       ; BI_global_get glob_tmp1
@@ -557,64 +562,339 @@ Definition div21_loop_body :=
       [ ]
   ].
 
-Definition translate_primitive_ternary_op op_name x y z : error (list basic_instruction) :=
-  if Kername.eqb op_name primInt63Diveucl_21 then
-    Ret (load_local_i64 z ++
-         [ BI_const_num maxuint63
-         ; BI_binop T_i64 (Binop_i BOI_and)
-         ; BI_global_set glob_tmp4
-         ] ++
-         load_local_i64 x ++
-         [ BI_const_num maxuint63
-         ; BI_binop T_i64 (Binop_i BOI_and)
-         ; BI_global_set glob_tmp1
-         ] ++
-         [ BI_global_get glob_tmp4
-         ; BI_global_get glob_tmp1
-         ; BI_relop T_i64 (Relop_i (ROI_le SX_U))
-         ; BI_if (BT_valtype (Some (T_num T_i32)))
-             ([ BI_const_num (nat_to_i64val 0) ; BI_global_set glob_tmp1 ] ++ make_product glob_tmp1 glob_tmp1)
-             (load_local_i64 y ++
-              [ BI_global_set glob_tmp2
-              ; BI_const_num (nat_to_i64val 0)
-              ; BI_global_set glob_tmp3
-              ] ++ (List.flat_map (fun x => x) (List.repeat div21_loop_body 63)) ++
-              [ BI_global_get glob_tmp1
-              ; BI_const_num maxuint63
-              ; BI_binop T_i64 (Binop_i BOI_and)
-              ; BI_global_set glob_tmp1
-              ] ++ (make_product glob_tmp3 glob_tmp1))
-         ])
+Definition diveucl_21_instrs (xh xl y : localidx) : list basic_instruction :=
+  load_local_i64 y ++ [ BI_global_set glob_tmp4 ] ++
+    load_local_i64 xh ++ [ BI_global_set glob_tmp1 ] ++
+    [ BI_global_get glob_tmp4
+    ; BI_global_get glob_tmp1
+    ; BI_relop T_i64 (Relop_i (ROI_le SX_U))
+    ; BI_if (BT_valtype (Some (T_num T_i32)))
+        ([ BI_const_num 0%Z ; BI_global_set glob_tmp1 ] ++ make_product glob_tmp1 glob_tmp1)
+        (load_local_i64 xl ++
+           [ BI_global_set glob_tmp2
+           ; BI_const_num 0%Z
+           ; BI_global_set glob_tmp3
+           ] ++ (List.flat_map (fun x => x) (List.repeat diveucl_21_loop_body 63)) ++
+           [ BI_global_get glob_tmp1
+           ; BI_const_num maxuint63
+           ; BI_binop T_i64 (Binop_i BOI_and)
+           ; BI_global_set glob_tmp1
+           ] ++ (make_product glob_tmp3 glob_tmp1))
+    ].
 
-  else if Kername.eqb op_name primInt63Addmuldiv then
-    Ret (BI_global_get global_mem_ptr ::
-         load_local_i64 x ++
-         [ BI_const_num (nat_to_i64val 63)
-         ; BI_relop T_i64 (Relop_i (ROI_gt SX_U))
-         ; BI_if (BT_valtype (Some (T_num T_i64)))
-             [ BI_const_num (nat_to_i64val 0) ]
-             (* Compute x << z on the stack *)
-             (load_local_i64 y ++
-              load_local_i64 x ++
-              [ BI_binop T_i64 (Binop_i BOI_shl)
-              ; BI_const_num maxuint63
-              ; BI_binop T_i64 (Binop_i BOI_and)
-              ] ++
-              (* Put y on the stack *)
-              load_local_i64 z ++
-              (* Compute 63 - z on the stack *)
-              [ BI_const_num (nat_to_i64val 63) ] ++
-              load_local_i64 x ++
-              [ BI_binop T_i64 (Binop_i BOI_sub)
-              (* Compute y >> (63 - z) on the stack *)
-              ; BI_binop T_i64 (Binop_i (BOI_shr SX_U))
-              (* Finally, compute (x << z) | (y >> (63 - z)) on the stack *)
-              ; BI_binop T_i64 (Binop_i BOI_or)
-              ])
-         ; BI_store T_i64 None 2%N 0%N
-         ; BI_global_get global_mem_ptr
-         ] ++ increment_global_mem_ptr 8)
+
+Definition addmuldiv_instrs p x y :=
+  BI_global_get global_mem_ptr ::
+    load_local_i64 p ++
+    [ BI_const_num 63%Z
+    ; BI_relop T_i64 (Relop_i (ROI_gt SX_U))
+    ; BI_if (BT_valtype (Some (T_num T_i64)))
+        [ BI_const_num 0%Z ]
+        (* Compute x << p on the stack *)
+        (load_local_i64 x ++
+           load_local_i64 p ++
+           [ BI_binop T_i64 (Binop_i BOI_shl)
+           ; BI_const_num maxuint63
+           ; BI_binop T_i64 (Binop_i BOI_and)
+           ] ++
+           (* Put y on the stack *)
+           load_local_i64 y ++
+           (* Compute 63 - p on the stack *)
+           [ BI_const_num 63%Z ] ++
+           load_local_i64 p ++
+           [ BI_binop T_i64 (Binop_i BOI_sub)
+           (* Compute y >> (63 - p) on the stack *)
+           ; BI_binop T_i64 (Binop_i (BOI_shr SX_U))
+           (* Finally, compute (x << p) | (y >> (63 - p)) on the stack *)
+           ; BI_binop T_i64 (Binop_i BOI_or)
+           ])
+    ; BI_store T_i64 None 2%N 0%N
+    ; BI_global_get global_mem_ptr
+    ] ++ increment_global_mem_ptr 8.
+
+Definition translate_primitive_ternary_op op (x y z : localidx) : error (list basic_instruction) :=
+  match op with
+  | PrimInt63diveucl_21 => Ret (diveucl_21_instrs x y z)
+  | PrimInt63addmuldiv  => Ret (addmuldiv_instrs x y z)
+  | _ => Err "Unknown primitive ternary operator"
+  end.
+
+End TRANSLATION.
+
+Section WRAPPERS.
+
+(* **** Define LambdaANF wrapper functions for Coq's 63 bit integer operators  **** *)
+
+(* LambdaANF constructor values 'Vconstr t vs' hold the tag 't' of the constructor and a list of values 'vs'.
+   The tag is NOT the same as the ordinal used in the translation section above,
+   and the tag of a specific constructor is NOT guaranteed to always be the same,
+   it depends on the program being extracted.
+
+   For the proof, we define 'wrapper' functions for the primitive operators,
+   and for primitive operators that return a constructor value, the wrapper function is parameterized over the tags
+   since we don't know the concrete values of the tags.
+
+   For convenience, we define the tags as section variables.
+ *)
+Variables true_tag false_tag eq_tag lt_tag gt_tag c0_tag c1_tag pair_tag : ctor_tag.
+
+Definition LambdaANF_primInt_arith_fun (f : uint63 -> uint63 -> uint63) (x y : uint63) := Vprim (primInt (f x y)).
+
+Definition LambdaANF_primInt_bool_fun (f : uint63 -> uint63 -> bool) x y :=
+  if f x y then
+    Vconstr true_tag []
   else
-    Err ("Unknown primitive arithmetic operator: " ++ (Kernames.string_of_kername op_name))%bs.
+    Vconstr false_tag [].
 
-End PrimitiveOperators.
+Definition LambdaANF_primInt_compare_fun (f : uint63 -> uint63 -> comparison) x y :=
+  match f x y with
+  | Datatypes.Eq => Vconstr eq_tag []
+  | Datatypes.Lt => Vconstr lt_tag []
+  | Datatypes.Gt => Vconstr gt_tag []
+  end.
+
+Definition LambdaANF_primInt_carry_fun (f : uint63 -> uint63 -> carry uint63) x y :=
+  match f x y with
+  | C0 z => Vconstr c0_tag [ Vprim (primInt z) ]
+  | C1 z => Vconstr c1_tag [ Vprim (primInt z) ]
+  end.
+
+Definition LambdaANF_primInt_prod_fun (f : uint63 -> uint63 -> prod uint63 uint63) x y :=
+  let p := f x y in
+  Vconstr pair_tag [ Vprim (primInt (fst p)) ; Vprim (primInt (snd p)) ].
+
+Definition LambdaANF_primInt_unop_fun (f : uint63 -> uint63) x := Vprim (primInt (f x)).
+
+Definition LambdaANF_primInt_diveucl_21 xh xl y :=
+  let (q, r) := diveucl_21 xh xl y in
+  Vconstr pair_tag [ Vprim (primInt q) ; Vprim (primInt r) ].
+
+Definition LambdaANF_primInt_addmuldiv p x y := Vprim (primInt (addmuldiv p x y)).
+
+(* Define a partial function for applying a primitive operator.
+   The result is only defined if the operator is supported and the arguments
+   match the type of the Coq operator.
+   E.g 'add' has the type 'uint63 -> uint63 -> uint63' so the arguments must be
+   2 primitive integer values and the return value is a primitive integer. *)
+Definition apply_LambdaANF_primInt_operator op (vs : list val) : option val :=
+  match vs with
+  | [ Vprim (primInt x) ] =>
+      match op with
+      | PrimInt63head0 => Some (LambdaANF_primInt_unop_fun Uint63.head0 x)
+      | PrimInt63tail0 => Some (LambdaANF_primInt_unop_fun Uint63.tail0 x)
+      | _ => None
+      end
+  | [ Vprim (primInt x) ; Vprim (primInt y) ] =>
+      match op with
+      | PrimInt63add => Some (LambdaANF_primInt_arith_fun Uint63.add x y)
+      | PrimInt63sub => Some (LambdaANF_primInt_arith_fun Uint63.sub x y)
+      | PrimInt63mul => Some (LambdaANF_primInt_arith_fun Uint63.mul x y)
+      | PrimInt63div => Some (LambdaANF_primInt_arith_fun Uint63.div x y)
+      | PrimInt63mod => Some (LambdaANF_primInt_arith_fun Uint63.mod x y)
+      | PrimInt63lsl => Some (LambdaANF_primInt_arith_fun Uint63.lsl x y)
+      | PrimInt63lsr => Some (LambdaANF_primInt_arith_fun Uint63.lsr x y)
+      | PrimInt63land => Some (LambdaANF_primInt_arith_fun Uint63.land x y)
+      | PrimInt63lor => Some (LambdaANF_primInt_arith_fun Uint63.lor x y)
+      | PrimInt63lxor => Some (LambdaANF_primInt_arith_fun Uint63.lxor x y)
+      | PrimInt63eqb => Some (LambdaANF_primInt_bool_fun Uint63.eqb x y)
+      | PrimInt63ltb => Some (LambdaANF_primInt_bool_fun Uint63.ltb x y)
+      | PrimInt63leb => Some (LambdaANF_primInt_bool_fun Uint63.leb x y)
+      | PrimInt63compare => Some (LambdaANF_primInt_compare_fun Uint63.compare x y)
+      | PrimInt63addc => Some (LambdaANF_primInt_carry_fun Uint63.addc x y)
+      | PrimInt63addcarryc => Some (LambdaANF_primInt_carry_fun Uint63.addcarryc x y)
+      | PrimInt63subc => Some (LambdaANF_primInt_carry_fun Uint63.subc x y)
+      | PrimInt63subcarryc => Some (LambdaANF_primInt_carry_fun Uint63.subcarryc x y)
+      | PrimInt63mulc => Some (LambdaANF_primInt_prod_fun Uint63.mulc x y)
+      | PrimInt63diveucl => Some (LambdaANF_primInt_prod_fun Uint63.diveucl x y)
+      | _ => None
+      end
+  | [ Vprim (primInt x) ; Vprim (primInt y) ; Vprim (primInt z) ] =>
+      match op with
+      | PrimInt63diveucl_21 => Some (LambdaANF_primInt_diveucl_21 x y z)
+      | PrimInt63addmuldiv => Some (LambdaANF_primInt_addmuldiv x y z)
+      | _ => None
+      end
+  | _ => None
+  end.
+
+End WRAPPERS.
+
+(* Arguments to primitive operations can only be primInts
+   (Eventually adapt for floats) *)
+Lemma apply_primop_only_defined_on_primInts :
+  forall op vs v true_tag false_tag eq_tag lt_tag gt_tag c0_tag c1_tag pair_tag,
+    apply_LambdaANF_primInt_operator true_tag false_tag eq_tag lt_tag gt_tag c0_tag c1_tag pair_tag op vs = Some v ->
+    forall v',
+      List.In v' vs -> exists n, v' = Vprim (primInt n).
+Proof.
+  intros.
+  unfold apply_LambdaANF_primInt_operator in H.
+  destruct vs=>//. destruct vs; destruct v0=>//; destruct p =>//; destruct x =>//.
+  destruct H0=>//. now exists p.
+  destruct vs; destruct v1=>//; destruct p0 =>//; destruct x =>//.
+  destruct H0. now exists p. destruct H0. now exists p0. destruct H0.
+  destruct vs; destruct v0=>//; destruct p1 =>//; destruct x =>//.
+  destruct H0. now exists p. destruct H0. now exists p0. destruct H0. now exists p1. destruct H0.
+Qed.
+
+(* Well-formedness of the primitive function (and constructor) environment:
+   Applying a (supported) primitive operator evaluates to a (LambdaANF) value, 
+   and the constructor environment contains all constructors that may be returned,
+   and the constructors have the expected ordinals (i.e. the ones used in the translation section).
+ *)
+Definition prim_funs_env_wellformed (cenv : ctor_env) (penv : prim_env) (prim_funs : M.t (list val -> option val)) : Prop :=
+  forall p op_name s b n op f vs v,
+    M.get p penv = Some (op_name, s, b, n) ->       (* penv = primitive function environment obtained from previous pipeline stage *)
+    KernameMap.find op_name primop_map = Some op -> (* primop_map = environment of supported primitive operations *)
+    M.get p prim_funs = Some f ->                   (* from lambdaANF operational semantics *)
+    f vs = Some v ->
+    exists true_tag false_tag it_bool eq_tag lt_tag gt_tag it_comparison c0_tag c1_tag it_carry pair_tag it_prod,
+      (* This links operational semantics to primitive operators in penv *)
+      apply_LambdaANF_primInt_operator true_tag false_tag eq_tag lt_tag gt_tag c0_tag c1_tag pair_tag op vs = Some v
+      (* Constructor tags (bools, comparison, carry and prod) used by prim ops *)
+      /\ M.get true_tag cenv = Some (Build_ctor_ty_info (Common.BasicAst.nNamed "true") (Common.BasicAst.nNamed "bool") it_bool 0%N true_ord)
+      /\ M.get false_tag cenv = Some (Build_ctor_ty_info (Common.BasicAst.nNamed "false") (Common.BasicAst.nNamed "bool") it_bool 0%N false_ord)
+      /\ M.get eq_tag cenv = Some (Build_ctor_ty_info (Common.BasicAst.nNamed "Eq") (Common.BasicAst.nNamed "comparison") it_comparison 0%N Eq_ord)
+      /\ M.get lt_tag cenv = Some (Build_ctor_ty_info (Common.BasicAst.nNamed "Lt") (Common.BasicAst.nNamed "comparison") it_comparison 0%N Lt_ord)
+      /\ M.get gt_tag cenv = Some (Build_ctor_ty_info (Common.BasicAst.nNamed "Gt") (Common.BasicAst.nNamed "comparison") it_comparison 0%N Gt_ord)
+      /\ M.get c0_tag cenv = Some (Build_ctor_ty_info (Common.BasicAst.nNamed "C0") (Common.BasicAst.nNamed "carry") it_carry 1%N C0_ord)
+      /\ M.get c1_tag cenv = Some (Build_ctor_ty_info (Common.BasicAst.nNamed "C1") (Common.BasicAst.nNamed "carry") it_carry 1%N C1_ord)
+      /\ M.get pair_tag cenv = Some (Build_ctor_ty_info (Common.BasicAst.nNamed "pair") (Common.BasicAst.nNamed "prod") it_prod 1%N pair_ord).
+
+Lemma uint63_mod_modulus_id :
+  forall (x : uint63), Int64.Z_mod_modulus (to_Z x) = to_Z x.
+Proof.
+  intros.
+  rewrite Int64.Z_mod_modulus_id. reflexivity.
+  assert (0 <= to_Z x < wB)%Z by now apply to_Z_bounded.
+  assert (wB < Int64.modulus)%Z. unfold Int64.modulus, Int64.half_modulus, two_power_nat. cbn. lia. lia.
+Qed.
+
+Corollary uint63_unsigned_id : forall (x : uint63), Int64.unsigned (to_Z x) = to_Z x.
+Proof. intros; simpl; now rewrite uint63_mod_modulus_id. Qed.
+
+Lemma Z_bitmask_modulo_equivalent :
+  forall (n : Z), Z.land n maxuint63 = Z.modulo n wB.
+Proof.
+  intros; now (replace maxuint63 with (Z.ones 63); [rewrite Z.land_ones|cbn]).
+Qed.
+
+Lemma int64_bitmask_modulo :
+  forall (x : Z),  Int64.iand x maxuint63 = Z.modulo x wB.
+Proof.
+  intros.
+  unfold Int64.iand, Int64.and. simpl.
+  rewrite Int64.Z_mod_modulus_eq.
+  rewrite Int64.modulus_twice_half_modulus.
+  replace (Z.land (x mod (2 * Int64.half_modulus)) 9223372036854775807)
+    with (Z.modulo (x mod (2 * Int64.half_modulus)) Int64.half_modulus) by now rewrite Z_bitmask_modulo_equivalent.
+  now rewrite Zaux.Zmod_mod_mult.
+Qed.
+
+Lemma uint63_eq_int64_eq :
+  forall x y, to_Z x = to_Z y -> Int64.eq (to_Z x) (to_Z y) = true.
+Proof.
+  intros; unfold Int64.eq; rewrite H; now rewrite zeq_true.
+Qed.
+
+Lemma uint63_neq_int64_neq :
+  forall x y, to_Z x <> to_Z y -> Int64.eq (to_Z x) (to_Z y) = false.
+Proof.
+  intros; unfold Int64.eq; do 2 rewrite uint63_unsigned_id; now rewrite zeq_false.
+Qed.
+
+Lemma to_Z_neq_uint63_eqb_false :
+  forall x y, to_Z x <> to_Z y -> (x =? y)%uint63 = false.
+Proof.
+  intros; rewrite eqb_false_spec; intro Hcontra; now rewrite Hcontra in H.
+Qed.
+
+Local Ltac solve_arith_op d1 d2 spec :=
+  intros; unfold d1, d2; (repeat rewrite uint63_unsigned_id); (try rewrite int64_bitmask_modulo); now rewrite spec.
+
+(* Helper lemmas to show that the Wasm arithmetic is correct w.r.t. 63 bit arithmetic.
+   Helps prove that E.g. the instructions
+
+   i64.const x
+   i64.const y
+   i64.add
+   i64.const (2^63 - 1)
+   i64.and
+
+   reduce to
+
+   i64.const ((x + y) mod 2^63)
+ *)
+Lemma uint63_add_i64_add : forall x y, Int64.iand (Int64.iadd (to_Z x) (to_Z y)) maxuint63 = to_Z (x + y).
+Proof. solve_arith_op Int64.iadd Int64.add add_spec. Qed.
+
+Lemma uint63_sub_i64_sub : forall x y, Int64.iand (Int64.isub (to_Z x) (to_Z y)) maxuint63 = to_Z (x - y).
+Proof. solve_arith_op Int64.isub Int64.sub sub_spec. Qed.
+
+Lemma uint63_mul_i64_mul : forall x y, Int64.iand (Int64.imul (to_Z x) (to_Z y)) maxuint63 = to_Z (x * y).
+Proof. solve_arith_op Int64.imul Int64.mul mul_spec. Qed.
+
+Local Ltac solve_div_mod d1 d2 spec :=
+  intros; unfold d1, d2;
+  repeat rewrite uint63_unsigned_id;
+  rewrite spec;
+  now (replace Int64.zero with (Int64.repr (to_Z 0)); [rewrite uint63_neq_int64_neq|rewrite to_Z_0]).
+
+Lemma uint63_div_i64_div : forall x y,
+    to_Z y <> to_Z 0 -> Int64.idiv_u (to_Z x) (to_Z y) = Some (Int64.repr (to_Z (x / y))).
+Proof. solve_div_mod Int64.idiv_u Int64.divu div_spec. Qed.
+
+Lemma uint63_div0 : forall x y,
+    to_Z y = to_Z 0 -> to_Z (x / y) = to_Z 0.
+Proof.
+  intros; rewrite div_spec H to_Z_0; unfold Z.div, Z.div_eucl; now destruct (to_Z x).
+Qed.
+
+Lemma uint63_mod_i64_mod : forall x y,
+    to_Z y <> to_Z 0 -> Int64.irem_u (to_Z x) (to_Z y) = Some (Int64.repr (to_Z (x mod y))).
+Proof. solve_div_mod Int64.irem_u Int64.modu mod_spec. Qed.
+
+Lemma uint63_mod0 : forall x y,
+    to_Z y = to_Z 0 -> to_Z (x mod y) = to_Z x.
+Proof.
+  intros; rewrite mod_spec H to_Z_0; unfold Z.modulo, Z.div_eucl; now destruct (to_Z x).
+Qed.
+
+Lemma uint63_land_i64_and : forall x y, Int64.iand (to_Z x) (to_Z y) = to_Z (x land y).
+Proof. solve_arith_op Int64.iand Int64.and land_spec'. Qed.
+
+Lemma uint63_lor_i64_or : forall x y, Int64.ior (to_Z x) (to_Z y) = to_Z (x lor y).
+Proof. solve_arith_op Int64.ior Int64.or lor_spec'. Qed.
+
+Lemma uint63_lxor_i64_xor : forall x y, Int64.ixor (to_Z x) (to_Z y) = to_Z (x lxor y).
+Proof. solve_arith_op Int64.ixor Int64.xor lxor_spec'. Qed.
+
+
+Lemma lsl_bits_high : forall x y,
+    (to_Z 63 <= to_Z y)%Z ->
+    forall i, bit (x << y) i = false.
+Proof.
+  intros.
+  destruct (digits <=? i)%uint63 eqn:Hi.
+  now apply bit_M.
+  rewrite bit_lsl; unfold digits in *.
+  assert (to_Z i < to_Z 63)%Z as Hi1 by
+      now destruct (reflect_dec _ _ (lebP 63 i)) as [H'|H']; [rewrite (reflect_iff _ _ (lebP 63 i)) in H'|].
+  assert (to_Z i < to_Z y)%Z as Hi2 by now replace (to_Z 63) with 63%Z in *; [lia|cbn].
+  now replace (i <? y)%uint63 with true; [cbn|rewrite (reflect_iff _ _ (ltbP i y)) in Hi2].
+Qed.
+
+Lemma uint63_bits_inj_0 i : (forall j, bit i j = false) -> i = 0%uint63.
+Proof.
+  intros.
+  assert (forall n, bit i n = bit 0 n) by now intros; rewrite bit_0; apply H.
+  now apply bit_ext.
+Qed.
+
+Lemma lsl_M_r : forall x y,
+    (to_Z 63 <= to_Z y)%Z ->
+    to_Z (x << y) = to_Z 0.
+Proof.
+  intros;
+  now replace (x << y)%uint63 with 0%uint63;[reflexivity|rewrite (uint63_bits_inj_0 _ (lsl_bits_high x y H))].
+Qed.
